Upd

Opcodes.fst
@@ -9,14 +9,23 @@ module List = FStar.List.Tot
 
 (* 76 A9 14 ... 88 AC *)
 
-assume val equ: f : 'a -> s: 'a -> Tot (bool)
-
 
 (* 118 *)
-val op_dup :	st_before: stackBC 'a{Stack.length st_before > 0}  -> 
+
+
+val op_dup : #a: eqtype -> st_before: stackBC a{Stack.length st_before > 0 /\ Stack.capacity st_before > 0}  -> 
 				line_before: seq nat{Seq.length line_before > 0 /\ (Seq.head line_before = 118)}
-				-> Tot (st: stackBC 'a 
+				-> Tot (st: stackBC a 
 								{Stack.length st > 1 /\ 
-								equ Stack.index st 0 Stack.index st 1 /\ 
-								Stack.length st = Stack.length st_before + 1} * 
-				line : seq nat {Seq.length line = Seq.length line_before - 1 } )
+								(Stack.index st 0) = (Stack.index st 1) /\ 
+								Stack.length st = Stack.length st_before + 1}	* 
+						line : seq nat {Seq.length line = Seq.length line_before - 1 }) 
+
+let op_dup #a st_before line_before = 
+	let pop = Stack.pop st_before in 
+	let element = fst pop in 
+	let stack_after_pop = snd pop in 
+	let stack_push1 = Stack.push stack_after_pop element in 
+	let stack_push2 = Stack.push stack_push1 element in 
+	let line = Seq.tail line_before in (stack_push2, line)
+
