StackBC.fst
@@ -1,31 +1,70 @@
 module StackBC
 
-open FStar.List.Tot
+open FStar.Seq
 
-module L = FStar.List.Tot
+module Seq = FStar.Seq
 
-type stackBC 'a = 
-| Mk : elements: list 'a -> capacity: nat -> length : nat{length = L.length elements} -> stackBC 'a
+type stackBC (a:eqtype) = 
+| Mk : elem: seq a -> cap: nat -> len : nat{len = Seq.length elem} -> stackBC a
 
 
-val elements: st : stackBC 'a -> Tot(list 'a)
-let elements st = 
+val elements:  #a:eqtype ->  st : stackBC a -> Tot(seq a)
+let elements #a st = 
 	match st with 
 	| Mk el _ _ -> el
 
-val capacity: st : stackBC 'a  -> Tot(nat)
-let capacity st = 
+val capacity:  #a:eqtype->  st : stackBC a  -> Tot(nat)
+let capacity #a st = 
 	match st with 
 	| Mk _ capacity _ -> capacity
 
-val length: st : stackBC 'a -> Tot(nat)
-let length st = 
+val length: #a:eqtype ->  st : stackBC a -> Tot(nat)
+let length #a st = 
 	match st with 
 	| Mk _ _ length -> length
 
 
-val index : st: stackBC 'a -> counter:nat {length st > counter}  -> 'a
-let index st counter = 
+val index : #a:eqtype ->  st: stackBC a -> counter:nat {length st > counter}  -> Tot(a)
+let index #a st counter = 
 	let elements = elements st in 
-	L.index elements counter 
+	index elements counter 
 
+val head: #a: eqtype -> st: stackBC a {length st > 0}-> Tot (a)
+let head #a st = 
+	index st 0
+
+
+val push: #a:eqtype ->  st: stackBC a{capacity st > 0} -> element : a  -> 
+	Tot(st_new: stackBC a{
+		length  st_new = length st + 1   /\ 
+		head st_new = element /\ 
+		capacity st_new = capacity st -1 } )
+
+let push #a st element = 
+	let elem = elements st in 
+	let cap = capacity st in 
+	let len = length st in 
+	let elements_new = Seq.cons element elem in 
+	let cap_new = cap  - 1 in 
+	let len_new = len + 1 in 
+	Mk elements_new cap_new len_new
+
+val pop_elem:#a : eqtype ->  st: stackBC a {length st > 0} -> Tot(a)
+let pop_elem #a st  = 
+	index st 0	
+
+val pop_stack: #a : eqtype -> st: stackBC a {length st >0} -> Tot (st_new: stackBC a{length st_new = length st - 1 })
+let pop_stack #a st  = 
+	let elem = elements st in 
+	let cap = capacity st in 
+	let len = length st in 
+	let elements_new = Seq.tail elem in 
+	let cap_new = cap + 1 in 
+	let len_new = len - 1 in
+	Mk elements_new cap_new len_new
+
+val pop: #a : eqtype -> st: stackBC a {length st > 0} -> Tot(a * (st_new : stackBC a{length st_new = length st -1}))
+let pop #a st = 
+	let elem = pop_elem #a st in 
+	let stack = pop_stack #a st in 
+	(elem,stack)
